theories/Views/ProdView.v
@@ -30,11 +30,11 @@ Section ExprDInject.
 
   Let tyArr : typ -> typ -> typ := @typ2 _ _ _ Typ2_tyArr.
 
-  Global Instance Injective_exprD'_App tus tvs (e1 e2 : expr typ func) (t : typ)
+  Global Instance Injective_lambda_exprD_App tus tvs (e1 e2 : expr typ func) (t : typ)
          (v : exprT tus tvs (typD t)):
-    Injective (ExprDsimul.ExprDenote.exprD' tus tvs t (App e1 e2) = Some v) := {
-      result := exists u v1 v2, ExprDsimul.ExprDenote.exprD' tus tvs (tyArr u t) e1 = Some v1 /\
-                                ExprDsimul.ExprDenote.exprD' tus tvs u e2 = Some v2 /\
+    Injective (ExprDsimul.ExprDenote.lambda_exprD tus tvs t (App e1 e2) = Some v) := {
+      result := exists u v1 v2, ExprDsimul.ExprDenote.lambda_exprD tus tvs (tyArr u t) e1 = Some v1 /\
+                                ExprDsimul.ExprDenote.lambda_exprD tus tvs u e2 = Some v2 /\
                                 v = AbsAppI.exprT_App v1 v2;
       injection := fun H => _
     }.
@@ -44,8 +44,8 @@ Section ExprDInject.
     do 3 eexists; repeat split; eassumption.
   Defined.
 
-  Global Instance Injective_exprD'_Inj tus tvs (f : func) (t : typ) (v : exprT tus tvs (typD t)):
-    Injective (ExprDsimul.ExprDenote.exprD' tus tvs t (Inj f) = Some v) := {
+  Global Instance Injective_lambda_exprD_Inj tus tvs (f : func) (t : typ) (v : exprT tus tvs (typD t)):
+    Injective (ExprDsimul.ExprDenote.lambda_exprD tus tvs t (Inj f) = Some v) := {
       result := exists v', symAs f t = Some v' /\ v = fun _ _ => v';
       injection := fun H => _
     }.
